examples/lambda/barendregt/solvableScript.sml
@@ -660,6 +660,20 @@ Proof
  >> qabbrev_tac ‘Ms = GENLIST (\i. funpow K m I) n’
  >> Q.EXISTS_TAC ‘Ms’
  (* applying lameq_LAMl_appstar_ISUB *)
+ >> MATCH_MP_TAC lameq_TRANS
+ >> Q.EXISTS_TAC ‘(VAR y @* Ns) ISUB (ZIP (Ms,vs))’
+ >> CONJ_TAC >- cheat
+ >> REWRITE_TAC [ISUB_appstar]
+ >> Q.PAT_X_ASSUM ‘MEM y vs’ ((Q.X_CHOOSE_THEN ‘i’ STRIP_ASSUME_TAC) o
+                              (REWRITE_RULE [MEM_EL]))
+ >> qabbrev_tac ‘Ns' = MAP (\e. e ISUB ZIP (Ms,vs)) Ns’
+ >> Know ‘VAR y ISUB ZIP (Ms,vs) = EL i Ms’
+ >- (cheat)
+ >> Rewr'
+ >> Know ‘EL i Ms = funpow K m I’
+ >- (‘i < n’ by rw [Abbr ‘n’] \\
+     rw [Abbr ‘Ms’, EL_GENLIST])
+ >> Rewr'
  >> cheat
 QED
 
